src/Ex/Mesi/MesiInv.v
@@ -63,7 +63,9 @@ Section CoherenceUnit.
                     (rsUpFrom oidx, (MRs, mesiDownRsS))] msgs.
 
   Definition ObjInvalid0 :=
-    ost#[status] = mesiI /\ NoCohMsgs.
+    ost#[status] = mesiI /\
+    ost#[dir].(dir_st) <> mesiE /\
+    NoCohMsgs.
 
   Definition ObjInvRs :=
     MsgExistsSig (downTo oidx, (MRs, mesiInvRs)) msgs.
